data/computability/partrec.lean
@@ -1,0 +1,104 @@
+/-
+Copyright (c) 2018 Mario Carneiro. All rights reserved.
+Released under Apache 2.0 license as described in the file LICENSE.
+Author: Mario Carneiro
+
+The partial recursive functions are defined similarly to the primitive
+recursive functions, but now all functions are partial, implemented
+using the `roption` monad, and there is an additional operation, called
+μ-recursion, which performs unbounded minimization.
+-/
+import data.computability.primrec data.pfun
+
+namespace nat
+
+section rfind
+parameter (p : ℕ →. bool)
+
+private def lbp (m n : ℕ) : Prop := m = n + 1 ∧ ∀ k ≤ n, ff ∈ p k
+
+parameter (H : ∃ n, tt ∈ p n ∧ ∀ k < n, (p k).dom)
+
+private def wf_lbp : well_founded lbp :=
+⟨let ⟨n, pn⟩ := H in begin
+  suffices : ∀m k, n ≤ k + m → acc (lbp p) k,
+  { from λa, this _ _ (nat.le_add_left _ _) },
+  intros m k kn,
+  induction m with m IH generalizing k;
+    refine ⟨_, λ y r, _⟩; rcases r with ⟨rfl, a⟩,
+  { injection roption.mem_unique pn.1 (a _ kn) },
+  { exact IH _ (by rw nat.add_right_comm; exact kn) }
+end⟩
+
+protected def rfind_x : {n // tt ∈ p n ∧ ∀m < n, ff ∈ p m} :=
+suffices ∀ k, (∀n < k, ff ∈ p n) → {n // tt ∈ p n ∧ ∀m < n, ff ∈ p m},
+from this 0 (λ n, (nat.not_lt_zero _).elim),
+@well_founded.fix _ _ lbp wf_lbp begin
+  intros m IH al,
+  have pm : (p m).dom,
+  { rcases H with ⟨n, h₁, h₂⟩,
+    rcases lt_trichotomy m n with h₃|h₃|h₃,
+    { exact h₂ _ h₃ },
+    { rw h₃, exact h₁.fst },
+    { injection roption.mem_unique h₁ (al _ h₃) } },
+  cases e : (p m).get pm,
+  { suffices,
+    exact IH _ ⟨rfl, this⟩ (λ n h, this _ (le_of_lt_succ h)),
+    intros n h, cases lt_or_eq_of_le h with h h,
+    { exact al _ h },
+    { rw h, exact ⟨_, e⟩ } },
+  { exact ⟨m, ⟨_, e⟩, al⟩ }
+end
+
+protected def rfind : ℕ := nat.rfind_x.1
+
+protected theorem rfind_spec : tt ∈ p rfind := nat.rfind_x.2.1
+
+protected theorem rfind_min : ∀ {m : ℕ}, m < rfind → ff ∈ p m := nat.rfind_x.2.right
+
+protected theorem rfind_min' {m : ℕ} (h : tt ∈ p m) : rfind ≤ m :=
+le_of_not_gt $ λ l, bool.no_confusion $
+roption.mem_unique (rfind_min l) h
+
+end rfind
+
+inductive partrec : (ℕ →. ℕ) → Prop
+| zero : partrec (pure 0)
+| succ : partrec succ
+| left : partrec (λ n, n.unpair.1)
+| right : partrec (λ n, n.unpair.2)
+| pair {f g} : partrec f → partrec g → partrec (λ n, mkpair <$> f n <*> g n)
+| comp {f g} : partrec f → partrec g → partrec (λ n, g n >>= f)
+| prec {f g} : partrec f → partrec g → partrec (unpaired (λ z n,
+   n.elim (f z) (λ y IH, (mkpair z ∘ mkpair y) <$> IH >>= g)))
+| rfind {f} : partrec f → partrec (unpaired (λ z n,
+   ⟨_, nat.rfind (λ n, (λ m, m = 0) <$> f (mkpair z n))⟩))
+
+namespace partrec
+
+theorem of_eq {f g : ℕ →. ℕ} (hg : partrec g) (H : ∀ n, f n = g n) : partrec f :=
+(funext H : f = g).symm ▸ hg
+
+theorem prim {f : ℕ → ℕ} (hf : primrec f) : partrec f :=
+begin
+  induction hf,
+  case nat.primrec.zero { exact zero },
+  case nat.primrec.succ { exact succ },
+  case nat.primrec.left { exact left },
+  case nat.primrec.right { exact right },
+  case nat.primrec.pair : f g hf hg pf pg {
+    refine (pf.pair pg).of_eq (λ n, (roption.eq_some_of_mem _).symm),
+    simp [has_seq.seq] },
+  case nat.primrec.comp : f g hf hg pf pg {
+    refine (pf.comp pg).of_eq (λ n, (roption.eq_some_of_mem _).symm),
+    simp [has_seq.seq] },
+  case nat.primrec.prec : f g hf hg pf pg {
+    refine (pf.prec pg).of_eq (λ n, (roption.eq_some_of_mem _).symm),
+    simp,
+    induction n.unpair.2 with m IH, {simp},
+    simp, exact ⟨_, ⟨_, IH, rfl⟩, rfl⟩ },
+end
+
+end partrec
+
+end nat
